backend/Tailcallproof.v
@@ -1351,10 +1351,7 @@ Proof.
     erewrite (Mem.record_stack_block_nextblock _ _ _ H5).
     rewrite Mem.push_new_stage_nextblock.
     reflexivity.
-  + repeat rewrite_stack_blocks.
-    intros b0 INS [|[]]. subst. simpl in INS.
-    apply Mem.in_frames_valid in INS.
-    eapply Mem.fresh_block_alloc; eauto.
+  + repeat rewrite_stack_blocks. easy.
   + red; simpl. intros b0 [|[]]. simpl in *; subst.
     red; rewrite Mem.push_new_stage_nextblock.
     eapply Mem.valid_new_block; eauto.
@@ -1376,7 +1373,6 @@ Proof.
       unfold option_map, flat_frameinj in Gi.
       repeat destr_in Gi. omega.
     * repeat rewrite_stack_blocks.
-      erewrite Genv.init_mem_stack_adt; eauto.
       red; red; simpl; intros.
       assert (i2 <= 1)%nat.
       apply frame_at_pos_lt in FAP2. simpl in FAP2. omega.
